examples/Monad2/MonadExpr.v
@@ -1,0 +1,12 @@
+Require Import MirrorCore.SymI.
+Require Import MirrorCore.SymEnv.
+Require Import MirrorCore.Lambda.Expr.
+Require Export MirrorCore.Examples.Monad2.MonadTypes.
+Require Import MirrorCore.Examples.Monad2.MonadSym.
+
+Set Implicit Arguments.
+Set Strict Implicit.
+
+Definition mext : Type := (SymEnv.func + mfunc)%type.
+
+Definition mexpr := expr typ mext.
