theories/Lambda/ExprDI.v
@@ -1,0 +1,339 @@
+Require Import ExtLib.Core.RelDec.
+Require Import ExtLib.Structures.Monads.
+Require Import ExtLib.Data.HList.
+Require Import ExtLib.Data.List.
+Require Import ExtLib.Data.Fun.
+Require Import ExtLib.Data.Monads.OptionMonad.
+Require Import ExtLib.Tactics.
+Require Import MirrorCore.EnvI.
+Require Import MirrorCore.SymI.
+Require Import MirrorCore.ExprI.
+Require Import MirrorCore.Lambda.TypesI2.
+Require Import MirrorCore.Lambda.ExprCore.
+
+Set Implicit Arguments.
+Set Strict Implicit.
+
+Module Type ExprDenote.
+
+  Section with_types.
+    Context {typ : Type}.
+    Context {typD : list Type -> typ -> Type}.
+    Context {func : Type}.
+    Context {RType_typD : RType typD}.
+    Context {Typ2_Fun : Typ2 typD Fun}.
+    Context {RSym_func : RSym typD func}.
+
+    (** Reasoning principles **)
+    Context {RTypeOk_typD : @RTypeOk _ typD _}.
+    Context {Typ2Ok_Fun : Typ2Ok _ Typ2_Fun}.
+    Context {RSymOk_func : RSymOk RSym_func}.
+
+    Let typ_arr : typ -> typ -> typ := @typ2 _ _ _ _.
+    Let arr_match := @typ2_match _ _ _ _ .
+    Let typD_arr
+    : forall ts a b, typD ts (typ_arr a b) = (typD ts a -> typD ts b)
+      := @typ2_cast _ _ _ _.
+
+
+    Global Instance RelDec_Rty ts : RelDec (Rty ts) :=
+    { rel_dec := fun a b => match type_cast ts a b with
+                              | Some _ => true
+                              | None => false
+                            end }.
+
+    Global Instance RelDec_Correct_Rty ts : @RelDec_Correct _ (Rty ts) _.
+    Proof.
+      constructor. unfold rel_dec; simpl.
+      intros; consider (type_cast ts x y); intros.
+      split; auto. apply type_cast_total in H; eauto with typeclass_instances.
+      intuition.
+    Qed.
+
+    Definition Rcast T {ts a b} (pf : Rty ts a b) : T (typD ts a) -> T (typD ts b) :=
+      Relim T (Rsym pf).
+
+    Definition Rcast_val
+    : forall {ts a b} (pf : Rty ts a b), typD ts a -> typD ts b :=
+      @Rcast (fun T => T).
+
+    Section OpenT.
+      Variable ts : list Type.
+      Variables tus tvs : tenv typ.
+
+      Definition OpenT (T : Type) :=
+        hlist (typD ts) tus -> hlist (typD ts) tvs -> T.
+
+      Definition Open_UseV (n : nat) : option { t : typ & OpenT (typD ts t) } :=
+        bind (m := option)
+             (nth_error_get_hlist_nth _ tvs n)
+             (fun t_get =>
+                let '(existT t get) := t_get in
+                ret (@existT _ (fun t => OpenT (typD ts t)) t
+                             (fun us vs => get vs))).
+
+      Definition Open_UseU (n : nat) : option { t : typ & OpenT (typD ts t) } :=
+        bind (m := option)
+             (nth_error_get_hlist_nth _ tus n)
+             (fun t_get =>
+                let '(existT t get) := t_get in
+                ret (@existT _ (fun t => OpenT (typD ts t)) t
+                             (fun us vs => get us))).
+
+      Definition Open_App {t u}
+      : OpenT (typD ts (typ_arr t u)) -> OpenT (typD ts t) -> OpenT (typD ts u) :=
+        match eq_sym (typD_arr ts t u) in _ = T
+              return OpenT T -> OpenT (typD ts t) -> OpenT (typD ts u)
+        with
+          | eq_refl => fun f x => fun us vs => (f us vs) (x us vs)
+        end.
+
+      Definition Open_Inj {t} (val : typD ts t)
+      : OpenT (typD ts t) :=
+        fun _ _ => val.
+
+
+      (** Auxiliary definitions **)
+      Definition Open_GetUAs (n : nat) (t : typ) :
+        option (OpenT (typD ts t)) :=
+        bind (m := option)
+             (nth_error_get_hlist_nth (typD ts) tus n)
+             (fun t_get =>
+                let '(existT t' get) := t_get in
+                bind (m := option)
+                     (type_cast ts t' t)
+                     (fun cast =>
+                        ret (fun us vs => Rcast_val cast (get us)))).
+
+      Definition Open_GetVAs (n : nat) (t : typ) :
+        option (OpenT (typD ts t)) :=
+        bind (m := option)
+             (nth_error_get_hlist_nth (typD ts) tvs n)
+             (fun t_get =>
+                let '(existT t' get) := t_get in
+                bind (m := option)
+                     (type_cast ts t' t)
+                     (fun cast =>
+                        ret (fun us vs => Rcast_val cast (get vs)))).
+
+    End OpenT.
+
+    Definition Open_Abs {ts tus tvs t u}
+    : OpenT ts tus (t :: tvs) (typD ts u) ->
+      OpenT ts tus tvs (typD ts (typ_arr t u)) :=
+      match eq_sym (typD_arr ts t u) in _ = T
+            return OpenT ts tus (t :: tvs) (typD ts u) -> OpenT ts tus tvs T
+      with
+        | eq_refl => fun f => fun us vs x => f us (Hcons x vs)
+      end.
+
+
+    Definition funcAs {ts} (f : func) (t : typ) : option (typD ts t) :=
+      match typeof_sym f as Z
+            return Z = typeof_sym f -> option (typD ts t)
+      with
+        | None => fun _ => None
+        | Some T => fun pf =>
+                      match type_cast ts T t with
+                        | None => None
+                        | Some cast =>
+                          Rcast option cast
+                                (Some (match pf in _ = Z
+                                             return match Z with
+                                                      | Some t => typD nil t
+                                                      | None => unit
+                                                    end -> typD ts _
+                                       with
+                                         | eq_refl => fun x => type_weaken ts x
+                                       end (symD f)))
+                      end
+      end eq_refl.
+
+    Definition func_simul ts (f : func) : option { t : typ & typD ts t } :=
+      match typeof_sym f as Z
+            return Z = typeof_sym f -> option _
+      with
+        | None => fun _ => None
+        | Some T => fun pf =>
+                      Some (@existT _ _ T
+                                    (match pf in _ = Z
+                                           return match Z with
+                                                    | Some t => typD nil t
+                                                    | None => unit
+                                                  end -> typD ts _
+                                     with
+                                       | eq_refl => fun x => type_weaken ts x
+                                     end (symD f)))
+      end eq_refl.
+
+    Parameter exprD'
+    : forall {RType_typD : RType typD} {Typ2_Fun : Typ2 typD Fun}
+             {RSym_func : RSym typD func}
+             ts (tus tvs : tenv typ) (t : typ) (e : expr typ func),
+        option (OpenT ts tus tvs (typD ts t)).
+
+    Axiom exprD'_respects
+    : @RTypeOk _ typD _ -> Typ2Ok _ Typ2_Fun -> RSymOk RSym_func ->
+      forall ts tus tvs t t' e (pf : Rty ts t' t),
+        exprD' ts tus tvs t e =
+        Rcast (fun T => option (OpenT ts tus tvs T)) pf (exprD' ts tus tvs t' e).
+
+    Section typeof_expr.
+      Variable ts : list Type.
+      Variable tus : tenv typ.
+
+      Definition type_of_apply (tv x : typ) : option typ :=
+        arr_match (fun _ => option typ) ts tv
+                  (fun d r =>
+                     match type_cast ts d x with
+                       | Some _ => Some r
+                       | None => None
+                     end)
+                  None.
+
+      Fixpoint typeof_expr (tvs : tenv typ) (e : expr typ func)
+      : option typ :=
+        match e with
+        | Var x  => nth_error tvs x
+        | UVar x => nth_error tus x
+        | Inj f => typeof_sym f
+        | App e e' =>
+          match typeof_expr tvs e
+              , typeof_expr tvs e'
+          with
+            | Some tf , Some tx =>
+              type_of_apply tf tx
+            | _ , _ => None
+          end
+        | Abs t e =>
+          match typeof_expr (t :: tvs) e with
+            | None => None
+            | Some t' => Some (typ_arr t t')
+          end
+      end.
+    End typeof_expr.
+
+    Axiom exprD'_Var
+    : @RTypeOk _ typD _ -> Typ2Ok _ Typ2_Fun -> RSymOk RSym_func ->
+      forall ts tus tvs t v,
+        exprD' ts tus tvs t (Var v) =
+        bind (m := option)
+             (nth_error_get_hlist_nth (typD ts) tvs v)
+             (fun t_get =>
+                let '(existT t' get) := t_get in
+                bind (m := option)
+                     (type_cast ts t' t)
+                     (fun cast =>
+                        ret (fun us vs => Rcast_val cast (get vs)))).
+
+    Axiom exprD'_UVar
+    : @RTypeOk _ typD _ -> Typ2Ok _ Typ2_Fun -> RSymOk RSym_func ->
+      forall ts tus tvs t u,
+        exprD' ts tus tvs t (UVar u) =
+        bind (m := option)
+             (nth_error_get_hlist_nth (typD ts) tus u)
+             (fun t_get =>
+                let '(existT t' get) := t_get in
+                bind (m := option)
+                     (type_cast ts t' t)
+                     (fun cast =>
+                        ret (fun us vs => Rcast_val cast (get us)))).
+
+    Axiom exprD'_Inj
+    : @RTypeOk _ typD _ -> Typ2Ok _ Typ2_Fun -> RSymOk RSym_func ->
+      forall ts tus tvs t s,
+        exprD' ts tus tvs t (Inj s) =
+        bind (m := option)
+             (funcAs s t)
+             (fun val =>
+                ret (fun _ _ => val)).
+
+    Axiom exprD'_App
+    : @RTypeOk _ typD _ -> Typ2Ok _ Typ2_Fun -> RSymOk RSym_func ->
+      forall ts tus tvs t f x,
+        exprD' ts tus tvs t (App f x) =
+        bind (m := option)
+             (typeof_expr ts tus tvs x)
+             (fun t' =>
+                bind (exprD' ts tus tvs (typ_arr t' t) f)
+                     (fun f =>
+                        bind (exprD' ts tus tvs t' x)
+                             (fun x =>
+                                ret (Open_App f x)))).
+
+    Axiom exprD'_Abs
+    : @RTypeOk _ typD _ -> Typ2Ok _ Typ2_Fun -> RSymOk RSym_func ->
+      forall ts tus tvs t t' e,
+        exprD' ts tus tvs t (Abs t' e) =
+        arr_match (fun T => option (OpenT ts tus tvs T)) ts t
+                  (fun d r =>
+                     bind (m := option)
+                          (type_cast ts d t')
+                          (fun cast =>
+                             bind (m := option)
+                                  (exprD' ts tus (t' :: tvs) r e)
+                                  (fun val =>
+                                     ret (fun us vs x =>
+                                            val us (Hcons (Rcast_val cast x) vs)))))
+                  None.
+
+  End with_types.
+
+End ExprDenote.
+
+Module Type ExprFacts (ED : ExprDenote).
+
+  Section with_types.
+    Context {typ : Type}.
+    Context {typD : list Type -> typ -> Type}.
+    Context {RType_typD : RType typD}.
+    Context {Typ2_Fun : Typ2 typD Fun}.
+    Context {func : Type}.
+    Context {RSym_func : RSym typD func}.
+
+    (** Reasoning principles **)
+    Context {RTypeOk_typD : @RTypeOk _ typD _}.
+    Context {Typ2Ok_Fun : Typ2Ok _ Typ2_Fun}.
+    Context {RSymOk_func : RSymOk RSym_func}.
+
+    Axiom typeof_expr_weaken
+    : @RTypeOk _ typD _ -> Typ2Ok _ Typ2_Fun -> RSymOk RSym_func ->
+      forall ts tus tvs e t tus' tvs',
+        ED.typeof_expr ts tus tvs e = Some t ->
+        ED.typeof_expr ts (tus ++ tus') (tvs ++ tvs') e = Some t.
+
+    Axiom exprD'_weaken
+    : @RTypeOk _ typD _ -> Typ2Ok _ Typ2_Fun -> RSymOk RSym_func ->
+      forall ts tus tvs (e : expr typ func) t val tus' tvs',
+        ED.exprD' ts tus tvs t e = Some val ->
+        exists val',
+          ED.exprD' ts (tus ++ tus') (tvs ++ tvs') t e = Some val' /\
+          forall us vs us' vs',
+            val us vs = val' (hlist_app us us') (hlist_app vs vs').
+
+    Axiom exprD'_type_cast
+    : @RTypeOk _ typD _ -> Typ2Ok _ Typ2_Fun -> RSymOk RSym_func ->
+      forall ts tus tvs e t,
+        ED.exprD' ts tus tvs t e =
+        match ED.typeof_expr ts tus tvs e with
+          | None => None
+          | Some t' =>
+            match @type_cast _ typD _ ts t' t with
+              | None => None
+              | Some cast =>
+                match ED.exprD' ts tus tvs t' e with
+                  | None => None
+                  | Some x =>
+                    Some (fun us gs => ED.Rcast (fun x => x) cast (x us gs))
+                end
+            end
+        end.
+
+    Axiom typeof_expr_exprD'
+    : @RTypeOk _ typD _ -> Typ2Ok _ Typ2_Fun -> RSymOk RSym_func ->
+      forall ts tus tvs e t,
+        ED.typeof_expr ts tus tvs e = Some t ->
+        exists val,
+          ED.exprD' ts tus tvs t e = Some val.
+  End with_types.
+End ExprFacts.
